wip on allEntries log matching

raft-proofs/AllEntriesLogMatchingProof.v
@@ -1,9 +1,25 @@
 Require Import List.
+Import ListNotations.
 
 Require Import VerdiTactics.
+Require Import Util.
 Require Import Net.
+Require Import Omega.
+
 Require Import Raft.
 Require Import RaftRefinementInterface.
+Require Import CommonDefinitions.
+Require Import CommonTheorems.
+Require Import RefinementCommonTheorems.
+Require Import SpecLemmas.
+Require Import RefinementSpecLemmas.
+
+Require Import UpdateLemmas.
+Local Arguments update {_} {_} {_} _ _ _ _ : simpl never.
+
+Require Import AllEntriesLeaderSublogInterface.
+Require Import LeaderSublogInterface.
+Require Import RefinedLogMatchingLemmasInterface.
 
 Require Import AllEntriesLogMatchingInterface.
 
@@ -12,7 +28,242 @@ Section AllEntriesLogMatching.
   Context {orig_base_params : BaseParams}.
   Context {one_node_params : OneNodeParams orig_base_params}.
   Context {raft_params : RaftParams orig_base_params}.
+  Context {rri : raft_refinement_interface}.
+  Context {aelsi : allEntries_leader_sublog_interface}.
+  Context {lsi : leader_sublog_interface}.
+  Context {rlmli : refined_log_matching_lemmas_interface}.
+
+  Ltac update_destruct :=
+    match goal with
+      | [ |- context [ update _ ?y _ ?x ] ] => destruct (name_eq_dec y x)
+      | [ H : context [ update _ ?y _ ?x ] |- _ ] => destruct (name_eq_dec y x)
+    end.
+
+  Ltac start :=
+    red; unfold allEntries_log_matching; simpl; intros.
+
+  Ltac start_update :=
+    start;
+    repeat find_higher_order_rewrite; do 2 (update_destruct; rewrite_update); [| | |eauto].
+
+  Lemma allEntries_log_matching_init :
+    refined_raft_net_invariant_init allEntries_log_matching.
+  Proof.
+    start. contradiction.
+  Qed.
+
+  Definition leader_sublog (net : network) :=
+    forall leader e h,
+      type (snd (nwState net leader)) = Leader ->
+      In e (log (snd (nwState net h))) ->
+      eTerm e = currentTerm (snd (nwState net leader)) ->
+      In e (log (snd (nwState net leader))).
+
+  Lemma leader_sublog_invariant :
+    forall net,
+      refined_raft_intermediate_reachable net ->
+      leader_sublog net.
+  Admitted.
+
+  Lemma invalid_index :
+    forall net h e,
+      refined_raft_intermediate_reachable net ->
+      In e (log (snd (nwState net h))) ->
+      eIndex e = S (maxIndex (log (snd (nwState net h)))) ->
+      False.
+  Proof.
+    intros.
+    intro_refined_invariant entries_sorted_invariant.
+    find_apply_lem_hyp maxIndex_is_max; auto.
+    find_rewrite.
+    omega.
+  Qed.
+
+  Lemma allEntries_log_matching_client_request :
+    refined_raft_net_invariant_client_request allEntries_log_matching.
+  Proof.
+    start.
+    repeat find_higher_order_rewrite.
+    find_copy_apply_lem_hyp update_elections_data_client_request_log_allEntries.
+    intuition; simpl in *.
+    - do 2 (update_destruct; rewrite_update); simpl in *; subst; repeat find_rewrite; eauto.
+    - do 2 (update_destruct; rewrite_update); [| | |eauto]; simpl in *; subst;
+        break_exists; break_and; repeat find_rewrite; subst; simpl in *.
+      + intuition; subst; eauto; exfalso.
+        * intro_refined_invariant allEntries_leader_sublog_invariant.
+          eapply_prop_hyp allEntries_leader_sublog In; eauto.
+          find_reverse_rewrite. concludes.
+          repeat find_rewrite; eapply invalid_index; eauto.
+        * repeat find_rewrite; eapply invalid_index; eauto.
+      + intuition; subst; eauto; exfalso.
+        intro_refined_invariant leader_sublog_invariant.
+        eapply_prop_hyp leader_sublog In; eauto.
+        find_rewrite. concludes.
+        repeat find_rewrite; eapply invalid_index; eauto.
+      + intuition; subst; eauto; exfalso.
+        intro_refined_invariant allEntries_leader_sublog_invariant.
+        eapply_prop_hyp allEntries_leader_sublog In; eauto.
+        find_reverse_rewrite. concludes.
+        repeat find_rewrite; eapply invalid_index; eauto.
+  Qed.
+
+  Lemma allEntries_log_matching_unchanged :
+    forall net st' h gd d ps',
+      allEntries_log_matching net ->
+      (forall h' : Net.name, st' h' = update (nwState net) h (gd, d) h') ->
+      log d = log (snd (nwState net h)) ->
+      allEntries gd = allEntries (fst (nwState net h)) ->
+      allEntries_log_matching {| nwPackets := ps'; nwState := st' |}.
+  Proof.
+    unfold allEntries_log_matching. intros.
+    find_higher_order_rewrite.
+    do 2 (update_destruct; rewrite_update); simpl in *;
+      repeat find_rewrite; eauto.
+  Qed.
+
+  Ltac unchanged :=
+    red; intros; eapply allEntries_log_matching_unchanged; subst; eauto.
+
+  Lemma allEntries_log_matching_timeout :
+    refined_raft_net_invariant_timeout allEntries_log_matching.
+  Proof.
+    unchanged.
+    - eauto using handleTimeout_log_same.
+    - apply update_elections_data_timeout_allEntries.
+  Qed.
+
+  Lemma appendEntries_haveNewEntries_false :
+    forall net p t n pli plt es ci h e,
+      refined_raft_intermediate_reachable net ->
+      In p (nwPackets net) ->
+      pBody p = AppendEntries t n pli plt es ci ->
+      haveNewEntries (snd (nwState net h)) es = false ->
+      In e es ->
+      In e (log (snd (nwState net h))).
+  Proof.
+    intros.
+    unfold haveNewEntries in *. do_bool. intuition;
+      [unfold not_empty in *; break_match; subst; simpl in *; intuition; congruence|].
+    break_match; try congruence.
+    do_bool. find_apply_lem_hyp findAtIndex_elim. intuition.
+    assert (es <> nil) by (destruct es; subst; simpl in *; intuition; congruence).
+    find_eapply_lem_hyp maxIndex_non_empty.
+    break_exists. intuition.
+    find_copy_eapply_lem_hyp entries_sorted_nw_invariant; eauto.
+    match goal with
+      | H : In e es |- _ => copy_eapply maxIndex_is_max H; eauto
+    end.
+    repeat find_rewrite.
+    find_eapply_lem_hyp entries_match_nw_host_invariant; eauto.
+  Qed.
+
+  Lemma allEntries_log_matching_append_entries :
+    refined_raft_net_invariant_append_entries allEntries_log_matching.
+  Proof.
+    start_update.
+    - subst. eapply update_elections_data_appendEntries_log_allEntries with (h' := n) in H.
+      intuition; simpl in *.
+      + repeat find_rewrite. eauto.
+      + repeat find_rewrite. find_rewrite_lem map_app. find_apply_lem_hyp in_app_or.
+        break_or_hyp; [|eauto].
+        find_rewrite_lem map_of_map. simpl in *.
+        find_rewrite_lem map_id.
+        find_eapply_lem_hyp appendEntries_haveNewEntries_false; eauto.
+        eapply uniqueIndices_elim_eq; eauto.
+        apply sorted_uniqueIndices.
+        intro_refined_invariant entries_sorted_invariant.
+        auto.
+      + subst. repeat find_rewrite.
+        find_rewrite_lem map_app. find_apply_lem_hyp in_app_or.
+        break_or_hyp.
+        * find_rewrite_lem map_of_map. simpl in *. find_rewrite_lem map_id.
+          eapply uniqueIndices_elim_eq; eauto.
+          apply sorted_uniqueIndices.
+          intro_refined_invariant entries_sorted_nw_invariant.
+          eauto.
+        * admit.
+      + repeat find_rewrite.
+        find_rewrite_lem map_app. do 2 find_apply_lem_hyp in_app_or.
+        intuition.
+        * find_rewrite_lem map_of_map. simpl in *. find_rewrite_lem map_id.
+          eapply uniqueIndices_elim_eq; eauto.
+          apply sorted_uniqueIndices.
+          intro_refined_invariant entries_sorted_nw_invariant.
+          eauto.
+        * admit.
+        * find_rewrite_lem map_of_map. simpl in *. find_rewrite_lem map_id.
+          admit.
+        * find_apply_lem_hyp removeAfterIndex_in. eauto.
+    - admit.
+    - admit.
+  Admitted.
+
+  Lemma allEntries_log_matching_append_entries_reply :
+    refined_raft_net_invariant_append_entries_reply allEntries_log_matching.
+  Proof.
+    unchanged.
+    eauto using handleAppendEntriesReply_log.
+  Qed.
+
+  Lemma allEntries_log_matching_request_vote :
+    refined_raft_net_invariant_request_vote allEntries_log_matching.
+  Proof.
+    unchanged.
+    - eauto using handleRequestVote_log.
+    - apply update_elections_data_requestVote_allEntries.
+  Qed.
+
+  Lemma allEntries_log_matching_request_vote_reply :
+    refined_raft_net_invariant_request_vote_reply allEntries_log_matching.
+  Proof.
+    unchanged.
+    - eauto using handleRequestVoteReply_log.
+    - apply update_elections_data_requestVoteReply_allEntries.
+  Qed.
+
+  Lemma allEntries_log_matching_do_leader :
+    refined_raft_net_invariant_do_leader allEntries_log_matching.
+  Proof.
+  Admitted.
+
+  Lemma allEntries_log_matching_do_generic_server :
+    refined_raft_net_invariant_do_generic_server allEntries_log_matching.
+  Proof.
+  Admitted.
+
+  Lemma allEntries_log_matching_state_same_packet_subset :
+    refined_raft_net_invariant_state_same_packet_subset allEntries_log_matching.
+  Proof.
+  Admitted.
+
+  Lemma allEntries_log_matching_reboot :
+    refined_raft_net_invariant_reboot allEntries_log_matching.
+  Proof.
+  Admitted.
+
+  Lemma allEntries_log_matching_invariant :
+    forall net,
+      refined_raft_intermediate_reachable net ->
+      allEntries_log_matching net.
+  Proof.
+    intros.
+    apply refined_raft_net_invariant; auto.
+    - apply allEntries_log_matching_init.
+    - apply allEntries_log_matching_client_request.
+    - apply allEntries_log_matching_timeout.
+    - apply allEntries_log_matching_append_entries.
+    - apply allEntries_log_matching_append_entries_reply.
+    - apply allEntries_log_matching_request_vote.
+    - apply allEntries_log_matching_request_vote_reply.
+    - apply allEntries_log_matching_do_leader.
+    - apply allEntries_log_matching_do_generic_server.
+    - apply allEntries_log_matching_state_same_packet_subset.
+    - apply allEntries_log_matching_reboot.
+  Qed.
+
 
   Instance aelmi : allEntries_log_matching_interface.
-  Admitted.
+  Proof.
+    constructor. exact allEntries_log_matching_invariant.
+  Qed.
 End AllEntriesLogMatching.
